Add definition of SmallStep and related predicates (#2)
Added:
- HeadSmallStep (step without context)
- SmallStep (step with context)
- SmallStep (potentially multiple steps with context)

LocalLang/Semantics.lean
@@ -1,12 +1,36 @@
 import LocalLang.AST
+import LocalLang.Evaluator
+import LocalLang.Ctx
+import Mathlib.Logic.Relation
 
--- TODO: define
-inductive SmallStep (defs : Definitions) : Expr → Expr → Prop where
+-- for rewriting (.funCall f es) in terms of let
+def letin_chain (vars : List (String × Expr)) (e : Expr) : Expr :=
+  vars.foldl (fun e' (x, xe) => .letIn x xe e') e
 
--- TODO: define
-inductive SmallSteps (defs : Definitions) : Expr → Expr → Prop where
+inductive HeadSmallStep (defs : Definitions) : Env → Expr → Expr → Prop where
+  | var_step : V[x]? = some n →
+      HeadSmallStep defs V (.var x) (.const n)
+  | bin_op_step {op : BinOp} :
+      HeadSmallStep defs V (.binOp op (.const e₁) (.const e₂)) (.const (op.eval e₁ e₂))
+  | letin_const_step {name : String} {val n : ℕ} :
+      HeadSmallStep defs V (.letIn name (.const val) (.const n)) (.const n)
+  | fun_step (f : String) (es : List Expr)
+      (Hf : f ∈ defs) (Hpn : defs[f].parameters.length = es.length) :
+      HeadSmallStep defs V (.funCall f es) (letin_chain (defs[f].parameters.zip es) defs[f].body)
+
+inductive SmallStep (defs : Definitions) : Env → Expr → Expr → Prop where
+  | ctx_step (ctx : Ctx) (V : Env) : HeadSmallStep defs (ctx.updateEnv V) e₁ e₂ →
+      SmallStep defs V (ctx.fill e₁) (ctx.fill e₂)
+
+abbrev SmallSteps (defs : Definitions) (env : Env) : Expr → Expr → Prop :=
+  Relation.ReflTransGen (SmallStep defs env)
+
+def SmallSteps.single {defs : Definitions} {env : Env} :
+    SmallStep defs env e₁ e₂ → SmallSteps defs env e₁ e₂ := by
+  intro step
+  exact Relation.ReflTransGen.single step
 
 -- TODO: prove
 theorem smallSteps_diamond {defs : Definitions} {e₁ e₂ e₃ : Expr}
-  (HA : SmallSteps defs e₁ e₂) (HB : SmallSteps defs e₁ e₃)
-  :  ∃ e₄, SmallSteps defs e₂ e₄ ∧ SmallSteps defs e₃ e₄ := sorry
+  (HA : SmallSteps defs V e₁ e₂) (HB : SmallSteps defs V e₁ e₃)
+  :  ∃ e₄, SmallSteps defs V e₂ e₄ ∧ SmallSteps defs V e₃ e₄ := sorry
