LocalLang/Ctx.lean
@@ -1,0 +1,24 @@
+import LocalLang.AST
+
+inductive Ctx : Type where
+  | hole : Ctx
+  | binOpLhs : Ctx → BinOp → Expr → Ctx
+  | binOpRhs : ℕ → BinOp → Ctx → Ctx
+  | letInExpr : String → Ctx → Expr → Ctx
+  | letInBody : String → ℕ → Ctx → Ctx
+
+abbrev Env := Std.HashMap String ℕ
+
+def Ctx.fill (e : Expr) : Ctx → Expr
+  | hole => e
+  | binOpLhs ctx op e' => Expr.binOp op (ctx.fill e) e'
+  | binOpRhs n op ctx => Expr.binOp op (.const n) (ctx.fill e)
+  | letInExpr x ctx e' => .letIn x (ctx.fill e) e'
+  | letInBody x n ctx => .letIn x (.const n) (ctx.fill e)
+
+def Ctx.updateEnv (env : Env) : Ctx → Env
+  | hole => env
+  | binOpLhs ctx _ _ => ctx.updateEnv env
+  | binOpRhs _ _ ctx => ctx.updateEnv env
+  | letInExpr _ ctx _ => ctx.updateEnv env
+  | letInBody x n ctx => ctx.updateEnv (env.insert x n)
