LocalLang/TypingGuarantees.lean
@@ -4,8 +4,9 @@ import LocalLang.Types
 import LocalLang.Typing
 
 -- TODO: prove
+-- TODO: V and Γ should be related
 theorem preservation (Γ : TypeContext) (e e' : Expr) (ty : LLType) (defs : Definitions)
-  : TypeJdg Γ e ty → SmallStep defs e e' → TypeJdg Γ e' ty := sorry
+  : TypeJdg Γ e ty → SmallStep defs V e e' → TypeJdg Γ e' ty := sorry
 
 -- Progress: if TypeJdg Γ e ty, then e can take a step.
 -- TODO: formalize
